@base <https://raw.githubusercontent.com/energy-domain/ontology-tests/main/001/01_base/> .
@prefix : <https://raw.githubusercontent.com/energy-domain/ontology-tests/main/001/01_base/> .
@prefix owl: <http://www.w3.org/2002/07/owl#> .
@prefix rdf: <http://www.w3.org/1999/02/22-rdf-syntax-ns#> .
@prefix rdfs: <http://www.w3.org/2000/01/rdf-schema#> .
@prefix dcterms: <http://purl.org/dc/terms/> .
@prefix skos: <http://www.w3.org/2004/02/skos/core#> .

##################################################
### Assets Taxonomy ###
##################################################
:Asset a owl:Class ;
    rdfs:label "Asset"@en ;
    rdfs:comment "Base class for all physical assets in the system."@en .

:Equipment a owl:Class ;
    rdfs:subClassOf :Asset ;
    dcterms:identifier "asset_equipment" ;
    skos:prefLabel "Equipment"@en ;
    skos:altLabel "Physical Equipment"@en ;
    skos:definition "Physical assets that perform specific operational functions in the system."@en ;
    :ifc_equivalentClass "IfcEquipment" ;
    :ifc_objectType "Equipment" ;
    :ifc_predefinedType "USERDEFINED" .

:TransportElement a owl:Class ;
    rdfs:subClassOf :Asset ;
    dcterms:identifier "asset_transport_element" ;
    skos:prefLabel "Transport Element"@en ;
    skos:altLabel "Transportation Component"@en ;
    skos:definition "Elements that facilitate the movement of fluids/materials between equipment."@en ;
    :ifc_equivalentClass "IfcDistributionFlowElement" ;
    :ifc_objectType "TransportElement" ;
    :ifc_predefinedType "USERDEFINED" .

:Pump a owl:Class ;
    rdfs:subClassOf :Equipment ;
    dcterms:identifier "asset_pump" ;
    skos:prefLabel "Pump"@en ;
    skos:altLabel "Fluid Pump"@en ;
    skos:definition "Mechanical device that moves fluids through pipes by mechanical action."@en ;
    :ifc_equivalentClass "IfcPump" .

:Tank a owl:Class ;
    rdfs:subClassOf :Equipment ;
    dcterms:identifier "asset_tank" ;
    skos:prefLabel "Tank"@en ;
    skos:altLabel "Storage Vessel"@en ;
    skos:definition "Container for storing liquids or gases at atmospheric or pressurized conditions."@en ;
    :ifc_equivalentClass "IfcTank" ;
    :ifc_objectType "Tank" ;
    :ifc_predefinedType "USERDEFINED" .

:Pipe a owl:Class ;
    rdfs:subClassOf :TransportElement ;
    dcterms:identifier "asset_pipe" ;
    skos:prefLabel "Pipe"@en ;
    skos:altLabel "Pipeline"@en ;
    skos:altLabel "Tubulação"@pt-br ;
    skos:definition "Cylindrical conduit that transports fluids between system components."@en ;
    :ifc_equivalentClass "IfcPipeSegment" .
